{
 "cells": [
  {
   "cell_type": "markdown",
   "metadata": {},
   "source": [
    "1. Draw in a single Geogebra notebook the following functions:\n",
    "   - $f(x) = x^2$\n",
    "   - $g(x) = \\sqrt{x}$\n",
    "   - $h(x) = \\frac{1}{x}$\n",
    "   - $j(x) = \\sin(x)$\n",
    "\n",
    "https://www.geogebra.org/calculator/ddjryem6\n",
    "\n",
    "\n",
    "---"
   ]
  },
  {
   "cell_type": "markdown",
   "metadata": {},
   "source": [
    "## Evaluating Functions at \\( x = 2 \\)\n",
    "\n",
    "Given the functions:\n",
    "\n",
    "$$\n",
    "\\begin{aligned}\n",
    "f(x) &= x^2 \\\\\n",
    "g(x) &= \\sqrt{x} \\\\\n",
    "h(x) &= \\frac{1}{x} \\\\\n",
    "j(x) &= \\sin(x)\n",
    "\\end{aligned}\n",
    "$$\n",
    "\n",
    "We evaluate them at \\( x = 2 \\):\n",
    "\n",
    "$$\n",
    "\\begin{aligned}\n",
    "f(2) &= 2^2 = 4 \\\\\n",
    "g(2) &= \\sqrt{2} \\approx 1.414 \\\\\n",
    "h(2) &= \\frac{1}{2} = 0.5 \\\\\n",
    "j(2) &= \\sin(2) \\approx 0.909\n",
    "\\end{aligned}\n",
    "$$\n",
    "\n",
    "---"
   ]
  },
  {
   "cell_type": "markdown",
   "metadata": {},
   "source": [
    "2. Let $f(x) = 3x - 1$ and $g(x) = \\sqrt{x}$. Find:\n",
    "   - $f(g(x))$\n",
    "   - $g(f(x))$\n",
    "   - $f(f(x))$\n",
    "   - $g(g(x))$"
   ]
  },
  {
   "cell_type": "markdown",
   "metadata": {},
   "source": [
    "## Function Composition\n",
    "\n",
    "Given the functions:\n",
    "\n",
    "$$\n",
    "\\begin{aligned}\n",
    "f(x) &= 3x - 1 \\\\\n",
    "g(x) &= \\sqrt{x}\n",
    "\\end{aligned}\n",
    "$$\n",
    "\n",
    "### Finding Compositions:\n",
    "\n",
    "#### 1. \\( f(g(x)) \\)\n",
    "\n",
    "$$\n",
    "\\begin{aligned}\n",
    "f(g(x)) &= f(\\sqrt{x}) \\\\\n",
    "&= 3\\sqrt{x} - 1\n",
    "\\end{aligned}\n",
    "$$\n",
    "\n",
    "#### 2. \\( g(f(x)) \\)\n",
    "\n",
    "$$\n",
    "\\begin{aligned}\n",
    "g(f(x)) &= g(3x - 1) \\\\\n",
    "&= \\sqrt{3x - 1}\n",
    "\\end{aligned}\n",
    "$$\n",
    "\n",
    "#### 3. \\( f(f(x)) \\)\n",
    "\n",
    "$$\n",
    "\\begin{aligned}\n",
    "f(f(x)) &= f(3x - 1) \\\\\n",
    "&= 3(3x - 1) - 1 \\\\\n",
    "&= 9x - 3 - 1 \\\\\n",
    "&= 9x - 4\n",
    "\\end{aligned}\n",
    "$$\n",
    "\n",
    "#### 4. \\( g(g(x)) \\)\n",
    "\n",
    "$$\n",
    "\\begin{aligned}\n",
    "g(g(x)) &= g(\\sqrt{x}) \\\\\n",
    "&= \\sqrt{\\sqrt{x}} \\\\\n",
    "&= x^{\\frac{1}{4}}\n",
    "\\end{aligned}\n",
    "$$\n",
    "\n",
    "\n",
    "https://www.geogebra.org/calculator/d9quxj3b\n",
    "\n",
    "\n",
    "---"
   ]
  },
  {
   "cell_type": "markdown",
   "metadata": {},
   "source": []
  },
  {
   "cell_type": "markdown",
   "metadata": {},
   "source": [
    "## Function Composition Check\n",
    "\n",
    "Given the functions:\n",
    "\n",
    "$$\n",
    "\\begin{aligned}\n",
    "f(x) &= e^x \\\\\n",
    "g(x) &= \\ln(x)\n",
    "\\end{aligned}\n",
    "$$\n",
    "\n",
    "### Checking Compositions:\n",
    "\n",
    "#### 1. \\( f(g(x)) \\)\n",
    "\n",
    "$$\n",
    "\\begin{aligned}\n",
    "f(g(x)) &= f(\\ln(x)) \\\\\n",
    "&= e^{\\ln(x)} \\\\\n",
    "&= x\n",
    "\\end{aligned}\n",
    "$$\n",
    "\n",
    "#### 2. \\( g(f(x)) \\)\n",
    "\n",
    "$$\n",
    "\\begin{aligned}\n",
    "g(f(x)) &= g(e^x) \\\\\n",
    "&= \\ln(e^x) \\\\\n",
    "&= x\n",
    "\\end{aligned}\n",
    "$$\n",
    "\n",
    "### Conclusion:\n",
    "\n",
    "We observe that:\n",
    "\n",
    "$$\n",
    "f(g(x)) = x \\quad \\text{and} \\quad g(f(x)) = x\n",
    "$$\n",
    "\n",
    "This means that the functions **\\( f(x) = e^x \\) and \\( g(x) = \\ln(x) \\) are inverses of each other.** Applying one function and then the other returns the original input \\( x \\).\n"
   ]
  },
  {
   "cell_type": "markdown",
   "metadata": {},
   "source": [
    "---\n",
    "\n",
    "4. We have function $f=\\{(1,7), (2,9), (3,11)\\}$. Give inverse function $f^{-1}$."
   ]
  },
  {
   "cell_type": "markdown",
   "metadata": {},
   "source": [
    "## Finding the Inverse of a Function\n",
    "\n",
    "Given the function:\n",
    "\n",
    "$$\n",
    "f = \\{(1,7), (2,9), (3,11)\\}\n",
    "$$\n",
    "\n",
    "To find the inverse function \\( f^{-1} \\), we swap each \\( (x, y) \\) pair to \\( (y, x) \\):\n",
    "\n",
    "$$\n",
    "f^{-1} = \\{(7,1), (9,2), (11,3)\\}\n",
    "$$\n",
    "\n",
    "### **Conclusion:**\n",
    "The inverse function \\( f^{-1} \\) consists of the ordered pairs:\n",
    "\n",
    "$$\n",
    "f^{-1} = \\{(7,1), (9,2), (11,3)\\}\n",
    "$$\n"
   ]
  },
  {
   "cell_type": "markdown",
   "metadata": {},
   "source": [
    "\n",
    "5. We have function $f=\\{(1,7), (2,7), (3,11)\\}$. Give inverse function $f^{-1}$."
   ]
  },
  {
   "cell_type": "markdown",
   "metadata": {},
   "source": [
    "## Finding the Inverse of a Function\n",
    "\n",
    "Given the function:\n",
    "\n",
    "$$\n",
    "f = \\{(1,7), (2,7), (3,11)\\}\n",
    "$$\n",
    "\n",
    "To find the inverse function \\( f^{-1} \\), we swap each \\( (x, y) \\) pair to \\( (y, x) \\):\n",
    "\n",
    "$$\n",
    "f^{-1} = \\{(7,1), (7,2), (11,3)\\}\n",
    "$$\n",
    "\n",
    "### **Important Observation:**\n",
    "The inverse relation \\( f^{-1} \\) is:\n",
    "\n",
    "$$\n",
    "\\{(7,1), (7,2), (11,3)\\}\n",
    "$$\n",
    "\n",
    "Since the value **7 maps to both 1 and 2**, the inverse **is not a function** because a function must have only one output for each input.\n",
    "\n",
    "### **Conclusion:**\n",
    "- The inverse relation exists, but it **is not a function** because one input (7) has multiple outputs (1 and 2).\n",
    "- For a function to have an inverse that is also a function, it must be **one-to-one (bijective)**, meaning each \\( x \\) must map to a unique \\( y \\).\n",
    "\n",
    "---"
   ]
  },
  {
   "cell_type": "markdown",
   "metadata": {},
   "source": [
    " We have function $f(x)= x-1$. Give inverse function $f^{-1}$. Show both functions on the same Geogebra notebook."
   ]
  },
  {
   "cell_type": "markdown",
   "metadata": {},
   "source": [
    "## Finding the Inverse of \\( f(x) = x - 1 \\)\n",
    "\n",
    "To find the inverse function \\( f^{-1}(x) \\), we follow these steps:\n",
    "\n",
    "1. Start with the given function:\n",
    "\n",
    "   $$\n",
    "   y = x - 1\n",
    "   $$\n",
    "\n",
    "2. Swap \\( x \\) and \\( y \\):\n",
    "\n",
    "   $$\n",
    "   x = y - 1\n",
    "   $$\n",
    "\n",
    "3. Solve for \\( y \\):\n",
    "\n",
    "   $$\n",
    "   \\begin{aligned}\n",
    "   x + 1 &= y \\\\\n",
    "   y &= x + 1\n",
    "   \\end{aligned}\n",
    "   $$\n",
    "\n",
    "Thus, the inverse function is:\n",
    "\n",
    "$$\n",
    "f^{-1}(x) = x + 1\n",
    "$$\n",
    "\n",
    "---\n",
    "\n",
    "### **Geogebra Inputs to Plot Both Functions**\n",
    "To visualize both \\( f(x) \\) and \\( f^{-1}(x) \\) in **Geogebra**, enter the following commands:\n",
    "\n",
    "\n",
    "\n",
    "\n",
    "\n",
    "\n",
    "\n",
    "\n",
    "https://www.geogebra.org/calculator/qqgxp25q"
   ]
  }
 ],
 "metadata": {
  "language_info": {
   "name": "python"
  }
 },
 "nbformat": 4,
 "nbformat_minor": 2
}
