{
 "cells": [
  {
   "cell_type": "markdown",
   "metadata": {},
   "source": [
    "1. Find the Taylor series and visualize obtained functions in Geogebra:\n",
    "   - $f(x) = \\cos(x)$ around $x = 0$ up to the 4th degree."
   ]
  },
  {
   "cell_type": "markdown",
   "metadata": {},
   "source": [
    "# Taylor Series Expansion of $f(x) = \\cos(x)$ at $x = 0$\n",
    "\n",
    "## 1. Taylor Series Definition\n",
    "The Taylor series of a function $f(x)$ centered at $x = a$ is given by:\n",
    "\n",
    "$$\n",
    "f(x) = \\sum_{n=0}^{\\infty} \\frac{f^{(n)}(a)}{n!} (x - a)^n\n",
    "$$\n",
    "\n",
    "For $f(x) = \\cos(x)$, we expand around $x = 0$.\n",
    "\n",
    "## 2. Compute the Taylor Series Terms\n",
    "The derivatives of $f(x) = \\cos(x)$ are:\n",
    "\n",
    "$$\n",
    "\\begin{aligned}\n",
    "f(x) &= \\cos(x), \\\\\n",
    "f'(x) &= -\\sin(x), \\\\\n",
    "f''(x) &= -\\cos(x), \\\\\n",
    "f'''(x) &= \\sin(x), \\\\\n",
    "f''''(x) &= \\cos(x)\n",
    "\\end{aligned}\n",
    "$$\n",
    "\n",
    "Evaluating at $x = 0$:\n",
    "\n",
    "$$\n",
    "\\begin{aligned}\n",
    "f(0) &= 1, \\\\\n",
    "f'(0) &= 0, \\\\\n",
    "f''(0) &= -1, \\\\\n",
    "f'''(0) &= 0, \\\\\n",
    "f''''(0) &= 1\n",
    "\\end{aligned}\n",
    "$$\n",
    "\n",
    "Thus, the Taylor series up to the 4th degree is:\n",
    "\n",
    "$$\n",
    "\\cos(x) \\approx 1 - \\frac{x^2}{2!} + \\frac{x^4}{4!}\n",
    "$$\n",
    "\n",
    "which simplifies to:\n",
    "\n",
    "$$\n",
    "\\cos(x) \\approx 1 - \\frac{x^2}{2} + \\frac{x^4}{24}\n",
    "$$\n",
    "\n",
    "## 3. Conclusion\n",
    "The 4th-degree Taylor approximation of $\\cos(x)$ around $x = 0$ is:\n",
    "\n",
    "$$\n",
    "T_4(x) = 1 - \\frac{x^2}{2} + \\frac{x^4}{24}\n",
    "$$\n",
    "\n",
    "\n",
    "https://www.geogebra.org/calculator/apfqrgaz\n",
    "\n",
    "\n",
    "---"
   ]
  },
  {
   "cell_type": "markdown",
   "metadata": {},
   "source": [
    "   - $h(x) = 1/(1-x)$ around $x = 0$ up to the 4rd degree."
   ]
  },
  {
   "cell_type": "markdown",
   "metadata": {},
   "source": [
    "# Taylor Series Expansion of $h(x) = \\frac{1}{1 - x}$ at $x = 0$\n",
    "\n",
    "## 1. Taylor Series Definition\n",
    "The Taylor series of a function $f(x)$ centered at $x = a$ is given by:\n",
    "\n",
    "$$\n",
    "f(x) = \\sum_{n=0}^{\\infty} \\frac{f^{(n)}(a)}{n!} (x - a)^n\n",
    "$$\n",
    "\n",
    "For $h(x) = \\frac{1}{1 - x}$, we expand around $x = 0$.\n",
    "\n",
    "## 2. Compute the Taylor Series Terms\n",
    "\n",
    "### **First few derivatives:**\n",
    "$$\n",
    "\\begin{aligned}\n",
    "h(x) &= (1 - x)^{-1}, \\\\\n",
    "h'(x) &= (1 - x)^{-2}, \\\\\n",
    "h''(x) &= 2(1 - x)^{-3}, \\\\\n",
    "h'''(x) &= 6(1 - x)^{-4}, \\\\\n",
    "h''''(x) &= 24(1 - x)^{-5}.\n",
    "\\end{aligned}\n",
    "$$\n",
    "\n",
    "### **Evaluate at $x = 0$:**\n",
    "$$\n",
    "\\begin{aligned}\n",
    "h(0) &= 1, \\\\\n",
    "h'(0) &= 1, \\\\\n",
    "h''(0) &= 2, \\\\\n",
    "h'''(0) &= 6, \\\\\n",
    "h''''(0) &= 24.\n",
    "\\end{aligned}\n",
    "$$\n",
    "\n",
    "Using the Taylor series formula:\n",
    "\n",
    "$$\n",
    "h(x) \\approx h(0) + h'(0) x + \\frac{h''(0)}{2!} x^2 + \\frac{h'''(0)}{3!} x^3 + \\frac{h''''(0)}{4!} x^4\n",
    "$$\n",
    "\n",
    "## 3. Substituting Values\n",
    "$$\n",
    "\\begin{aligned}\n",
    "h(x) &\\approx 1 + x + \\frac{2}{2!} x^2 + \\frac{6}{3!} x^3 + \\frac{24}{4!} x^4, \\\\\n",
    "&\\approx 1 + x + x^2 + x^3 + x^4.\n",
    "\\end{aligned}\n",
    "$$\n",
    "\n",
    "Thus, the **4th-degree Taylor series** of $h(x) = \\frac{1}{1 - x}$ around $x = 0$ is:\n",
    "\n",
    "$$\n",
    "h(x) \\approx 1 + x + x^2 + x^3 + x^4.\n",
    "$$\n",
    "\n",
    "This series is a well-known **geometric series expansion**:\n",
    "\n",
    "$$\n",
    "\\frac{1}{1 - x} = \\sum_{n=0}^{\\infty} x^n, \\quad \\text{for } |x| < 1.\n",
    "$$\n",
    "\n",
    "\n",
    "https://www.geogebra.org/calculator/fsjvtfy8\n",
    "\n",
    "\n",
    "---"
   ]
  },
  {
   "cell_type": "markdown",
   "metadata": {},
   "source": [
    "   - $g(x) = \\sin(x)$ around $x = \\pi$ up to the 4rd degree."
   ]
  },
  {
   "cell_type": "markdown",
   "metadata": {},
   "source": [
    "# Taylor Series Expansion of $g(x) = \\sin(x)$ at $x = \\pi$\n",
    "\n",
    "## 1. Taylor Series Definition\n",
    "The Taylor series of a function $f(x)$ centered at $x = a$ is given by:\n",
    "\n",
    "$$\n",
    "f(x) = \\sum_{n=0}^{\\infty} \\frac{f^{(n)}(a)}{n!} (x - a)^n\n",
    "$$\n",
    "\n",
    "For $g(x) = \\sin(x)$, we expand around $x = \\pi$.\n",
    "\n",
    "## 2. Compute the Taylor Series Terms\n",
    "\n",
    "### **First few derivatives:**\n",
    "$$\n",
    "\\begin{aligned}\n",
    "g(x) &= \\sin(x), \\\\\n",
    "g'(x) &= \\cos(x), \\\\\n",
    "g''(x) &= -\\sin(x), \\\\\n",
    "g'''(x) &= -\\cos(x), \\\\\n",
    "g''''(x) &= \\sin(x).\n",
    "\\end{aligned}\n",
    "$$\n",
    "\n",
    "### **Evaluate at $x = \\pi$:**\n",
    "$$\n",
    "\\begin{aligned}\n",
    "g(\\pi) &= \\sin(\\pi) = 0, \\\\\n",
    "g'(\\pi) &= \\cos(\\pi) = -1, \\\\\n",
    "g''(\\pi) &= -\\sin(\\pi) = 0, \\\\\n",
    "g'''(\\pi) &= -\\cos(\\pi) = 1, \\\\\n",
    "g''''(\\pi) &= \\sin(\\pi) = 0.\n",
    "\\end{aligned}\n",
    "$$\n",
    "\n",
    "Using the Taylor series formula:\n",
    "\n",
    "$$\n",
    "g(x) \\approx g(\\pi) + g'(\\pi) (x - \\pi) + \\frac{g''(\\pi)}{2!} (x - \\pi)^2 + \\frac{g'''(\\pi)}{3!} (x - \\pi)^3 + \\frac{g''''(\\pi)}{4!} (x - \\pi)^4\n",
    "$$\n",
    "\n",
    "## 3. Substituting Values\n",
    "$$\n",
    "\\begin{aligned}\n",
    "g(x) &\\approx 0 - (x - \\pi) + \\frac{0}{2!} (x - \\pi)^2 + \\frac{1}{3!} (x - \\pi)^3 + \\frac{0}{4!} (x - \\pi)^4, \\\\\n",
    "&\\approx -(x - \\pi) + \\frac{(x - \\pi)^3}{6}.\n",
    "\\end{aligned}\n",
    "$$\n",
    "\n",
    "Thus, the **4th-degree Taylor series** of $g(x) = \\sin(x)$ around $x = \\pi$ is:\n",
    "\n",
    "$$\n",
    "g(x) \\approx -(x - \\pi) + \\frac{(x - \\pi)^3}{6}.\n",
    "$$\n",
    "\n",
    "https://www.geogebra.org/calculator/jdm2qnxb"
   ]
  },
  {
   "cell_type": "markdown",
   "metadata": {},
   "source": [
    "---\n",
    "2. Find a tangent line $y = f'(x_0) (x-x_0) + f(x_0)$ to the function $f(x) = e^{\\sin(x)}$ at $x_0 = \\pi$."
   ]
  },
  {
   "cell_type": "markdown",
   "metadata": {},
   "source": [
    "# Finding the Tangent Line to $f(x) = e^{\\sin(x)}$ at $x_0 = \\pi$\n",
    "\n",
    "## 1. Tangent Line Formula\n",
    "The equation of a tangent line to a function $f(x)$ at $x = x_0$ is given by:\n",
    "\n",
    "$$\n",
    "y = f'(x_0) (x - x_0) + f(x_0)\n",
    "$$\n",
    "\n",
    "where:\n",
    "- $f(x)$ is the function,\n",
    "- $f'(x_0)$ is the derivative evaluated at $x_0$.\n",
    "\n",
    "## 2. Compute $f(x)$ and $f'(x)$\n",
    "\n",
    "Given:\n",
    "$$\n",
    "f(x) = e^{\\sin(x)}\n",
    "$$\n",
    "\n",
    "### **Derivative of $f(x)$**\n",
    "Using the chain rule:\n",
    "\n",
    "$$\n",
    "f'(x) = e^{\\sin(x)} \\cdot \\cos(x)\n",
    "$$\n",
    "\n",
    "### **Evaluate at $x_0 = \\pi$**\n",
    "Since:\n",
    "\n",
    "$$\n",
    "\\sin(\\pi) = 0, \\quad \\cos(\\pi) = -1\n",
    "$$\n",
    "\n",
    "we get:\n",
    "\n",
    "$$\n",
    "\\begin{aligned}\n",
    "f(\\pi) &= e^{\\sin(\\pi)} = e^0 = 1, \\\\\n",
    "f'(\\pi) &= e^{\\sin(\\pi)} \\cdot \\cos(\\pi) = e^0 \\cdot (-1) = -1.\n",
    "\\end{aligned}\n",
    "$$\n",
    "\n",
    "## 3. Tangent Line Equation\n",
    "Substituting into the tangent line formula:\n",
    "\n",
    "$$\n",
    "y = (-1)(x - \\pi) + 1\n",
    "$$\n",
    "\n",
    "which simplifies to:\n",
    "\n",
    "$$\n",
    "y = -x + \\pi + 1.\n",
    "$$\n",
    "\n",
    "Thus, the equation of the **tangent line** to $f(x) = e^{\\sin(x)}$ at $x_0 = \\pi$ is:\n",
    "\n",
    "$$\n",
    "y = -x + \\pi + 1.\n",
    "$$\n",
    "\n",
    "\n",
    "https://www.geogebra.org/calculator/ffadxcte"
   ]
  }
 ],
 "metadata": {
  "language_info": {
   "name": "python"
  }
 },
 "nbformat": 4,
 "nbformat_minor": 2
}
