{
 "cells": [
  {
   "cell_type": "markdown",
   "metadata": {},
   "source": [
    "### Equation of a Circle\n",
    "\n",
    "1. **General Equation of a Circle**:\n",
    "   The general equation of a circle with center \\( (h, k) \\) and radius \\( r \\) is given by:\n",
    "   $$\n",
    "   (x - h)^2 + (y - k)^2 = r^2\n",
    "   $$\n",
    "\n",
    "2. **Substitute the Given Values**:\n",
    "   Here, the center is \\( A(1, 2) \\), so \\( h = 1 \\) and \\( k = 2 \\), and the radius is \\( r = 3 \\). Substituting these values into the general equation:\n",
    "   $$\n",
    "   (x - 1)^2 + (y - 2)^2 = 3^2\n",
    "   $$\n",
    "\n",
    "3. **Simplify the Equation**:\n",
    "   Simplifying the equation:\n",
    "   $$\n",
    "   (x - 1)^2 + (y - 2)^2 = 9\n",
    "   $$\n",
    "\n",
    "Thus, the equation of the circle is:\n",
    "$$\n",
    "(x - 1)^2 + (y - 2)^2 = 9\n",
    "$$\n",
    "\n",
    "https://www.geogebra.org/calculator/ar9debwm\n",
    "\n",
    "---\n"
   ]
  },
  {
   "cell_type": "markdown",
   "metadata": {},
   "source": [
    "### Equation of a Parabola\n",
    "\n",
    "1. **General Form of the Parabola**:\n",
    "   The equation of a parabola that intersects the \\( O_x \\)-axis at points \\( x = 2 \\) and \\( x = 4 \\) is of the form:\n",
    "   $$\n",
    "   y = a(x - 2)(x - 4)\n",
    "   $$\n",
    "\n",
    "2. **Substitute the Known Point**:\n",
    "   The parabola passes through the point \\( (3, 1) \\), so substitute \\( x = 3 \\) and \\( y = 1 \\) into the equation to find \\( a \\):\n",
    "   $$\n",
    "   1 = a(3 - 2)(3 - 4)\n",
    "   $$\n",
    "\n",
    "3. **Solve for \\( a \\)**:\n",
    "   Simplifying the equation:\n",
    "   $$\n",
    "   1 = a(1)(-1)\n",
    "   $$\n",
    "   $$\n",
    "   1 = -a\n",
    "   $$\n",
    "   So, \\( a = -1 \\).\n",
    "\n",
    "4. **Final Equation of the Parabola**:\n",
    "   Substituting \\( a = -1 \\) into the equation:\n",
    "   $$\n",
    "   y = -1(x - 2)(x - 4)\n",
    "   $$\n",
    "\n",
    "Thus, the equation of the parabola is:\n",
    "$$\n",
    "y = -(x - 2)(x - 4)\n",
    "$$\n",
    "\n",
    "https://www.geogebra.org/calculator/gw3a8sr7\n",
    "\n",
    "---"
   ]
  },
  {
   "cell_type": "markdown",
   "metadata": {},
   "source": [
    "### Find the Center of the Ellipse\n",
    "\n",
    "We are given the equation of the ellipse:\n",
    "\n",
    "$$\n",
    "x^2 + 4y^2 - 4x - 16y + 16 = 0\n",
    "$$\n",
    "\n",
    "1. **Rearrange the equation**:\n",
    "   Group the \\( x \\)-terms and \\( y \\)-terms:\n",
    "   $$\n",
    "   (x^2 - 4x) + 4(y^2 - 4y) = -16\n",
    "   $$\n",
    "\n",
    "2. **Complete the square** for the \\( x \\)-terms and \\( y \\)-terms:\n",
    "\n",
    "   - For \\( x^2 - 4x \\), the square of half of \\( -4 \\) is \\( (-2)^2 = 4 \\), so add and subtract 4.\n",
    "   - For \\( y^2 - 4y \\), the square of half of \\( -4 \\) is \\( (-2)^2 = 4 \\), so add and subtract 4, but remember to multiply by 4 because of the coefficient 4 in front of \\( y^2 \\).\n",
    "\n",
    "   So, the equation becomes:\n",
    "   $$\n",
    "   (x^2 - 4x + 4) + 4(y^2 - 4y + 4) = -16 + 4 + 16\n",
    "   $$\n",
    "\n",
    "3. **Simplify the equation**:\n",
    "   $$\n",
    "   (x - 2)^2 + 4(y - 2)^2 = 4\n",
    "   $$\n",
    "\n",
    "4. **Rewrite the equation in standard form**:\n",
    "   Divide through by 4 to get:\n",
    "   $$\n",
    "   \\frac{(x - 2)^2}{4} + (y - 2)^2 = 1\n",
    "   $$\n",
    "\n",
    "5. **Identify the center**:\n",
    "   The center of the ellipse is given by the values of \\( h \\) and \\( k \\) in the standard form \\( \\frac{(x - h)^2}{a^2} + \\frac{(y - k)^2}{b^2} = 1 \\). In this case, the center is \\( (h, k) = (2, 2) \\).\n",
    "\n",
    "### Final Answer:\n",
    "The center of the ellipse is \\( (2, 2) \\).\n",
    "\n",
    "https://www.geogebra.org/calculator/r3pr7ffh\n",
    "\n",
    "---"
   ]
  },
  {
   "cell_type": "markdown",
   "metadata": {},
   "source": [
    "### Problem: Find the slope \\( m \\) of the line \\( y = mx - 5 \\) that is tangent to the circle \\( x^2 + y^2 = 1 \\).\n",
    "\n",
    "1. **Equation of the Circle**:\n",
    "   The equation of the circle is:\n",
    "   $$\n",
    "   x^2 + y^2 = 1\n",
    "   $$\n",
    "\n",
    "2. **Equation of the Line**:\n",
    "   The equation of the line is:\n",
    "   $$\n",
    "   y = mx - 5\n",
    "   $$\n",
    "\n",
    "3. **Substitute the equation of the line into the equation of the circle**:\n",
    "   Since the line is tangent to the circle, it touches the circle at exactly one point. We substitute \\( y = mx - 5 \\) into the circle's equation:\n",
    "   $$\n",
    "   x^2 + (mx - 5)^2 = 1\n",
    "   $$\n",
    "\n",
    "4. **Expand the equation**:\n",
    "   Expanding \\( (mx - 5)^2 \\) gives:\n",
    "   $$\n",
    "   x^2 + (m^2x^2 - 10mx + 25) = 1\n",
    "   $$\n",
    "\n",
    "5. **Simplify the equation**:\n",
    "   Combine like terms:\n",
    "   $$\n",
    "   (1 + m^2)x^2 - 10mx + 25 = 1\n",
    "   $$\n",
    "   Simplifying further:\n",
    "   $$\n",
    "   (1 + m^2)x^2 - 10mx + 24 = 0\n",
    "   $$\n",
    "\n",
    "6. **Condition for tangency**:\n",
    "   For the line to be tangent to the circle, the quadratic equation must have exactly one solution. This occurs when the discriminant is zero. The discriminant \\( \\Delta \\) of a quadratic equation \\( ax^2 + bx + c = 0 \\) is given by:\n",
    "   $$\n",
    "   \\Delta = b^2 - 4ac\n",
    "   $$\n",
    "\n",
    "   For the quadratic equation \\( (1 + m^2)x^2 - 10mx + 24 = 0 \\), we have:\n",
    "   - \\( a = 1 + m^2 \\)\n",
    "   - \\( b = -10m \\)\n",
    "   - \\( c = 24 \\)\n",
    "\n",
    "   The discriminant is:\n",
    "   $$\n",
    "   \\Delta = (-10m)^2 - 4(1 + m^2)(24)\n",
    "   $$\n",
    "\n",
    "7. **Solve for \\( m \\)**:\n",
    "   Set the discriminant equal to zero:\n",
    "   $$\n",
    "   100m^2 - 4(1 + m^2)(24) = 0\n",
    "   $$\n",
    "   Simplify the equation:\n",
    "   $$\n",
    "   100m^2 - 96 - 96m^2 = 0\n",
    "   $$\n",
    "   Combine like terms:\n",
    "   $$\n",
    "   4m^2 = 96\n",
    "   $$\n",
    "   Solve for \\( m \\):\n",
    "   $$\n",
    "   m^2 = 24\n",
    "   $$\n",
    "   $$\n",
    "   m = \\sqrt{24} = 2\\sqrt{6}\n",
    "   $$\n",
    "\n",
    "### Final Answer:\n",
    "The slope of the tangent line is:\n",
    "$$\n",
    "m = 2\\sqrt{6}\n",
    "$$\n",
    "\n",
    "https://www.geogebra.org/calculator/rrykf63g\n",
    "\n",
    "---"
   ]
  },
  {
   "cell_type": "markdown",
   "metadata": {},
   "source": [
    "### Problem: Find the intersection points of the hyperbola \\( x^2 - y^2 = 1 \\) with the ellipse \\( x^2 + 4y^2 = 6 \\).\n",
    "\n",
    "1. **Equations of the Hyperbola and the Ellipse**:\n",
    "   The equation of the hyperbola is:\n",
    "   $$\n",
    "   x^2 - y^2 = 1\n",
    "   $$\n",
    "   The equation of the ellipse is:\n",
    "   $$\n",
    "   x^2 + 4y^2 = 6\n",
    "   $$\n",
    "\n",
    "2. **Substitute the equation of the hyperbola into the equation of the ellipse**:\n",
    "   To find the intersection points, substitute \\( x^2 = y^2 + 1 \\) from the hyperbola's equation into the ellipse's equation:\n",
    "   $$\n",
    "   (y^2 + 1) + 4y^2 = 6\n",
    "   $$\n",
    "\n",
    "3. **Simplify the equation**:\n",
    "   Combine like terms:\n",
    "   $$\n",
    "   y^2 + 1 + 4y^2 = 6\n",
    "   $$\n",
    "   $$\n",
    "   5y^2 + 1 = 6\n",
    "   $$\n",
    "\n",
    "4. **Solve for \\( y^2 \\)**:\n",
    "   Subtract 1 from both sides:\n",
    "   $$\n",
    "   5y^2 = 5\n",
    "   $$\n",
    "   Divide by 5:\n",
    "   $$\n",
    "   y^2 = 1\n",
    "   $$\n",
    "\n",
    "5. **Find \\( y \\)**:\n",
    "   Take the square root of both sides:\n",
    "   $$\n",
    "   y = \\pm 1\n",
    "   $$\n",
    "\n",
    "6. **Find the corresponding \\( x \\) values**:\n",
    "   Substitute \\( y = 1 \\) and \\( y = -1 \\) back into the equation of the hyperbola \\( x^2 - y^2 = 1 \\).\n",
    "\n",
    "   - For \\( y = 1 \\):\n",
    "     $$\n",
    "     x^2 - 1^2 = 1 \\quad \\Rightarrow \\quad x^2 - 1 = 1 \\quad \\Rightarrow \\quad x^2 = 2 \\quad \\Rightarrow \\quad x = \\pm \\sqrt{2}\n",
    "     $$\n",
    "\n",
    "   - For \\( y = -1 \\):\n",
    "     $$\n",
    "     x^2 - (-1)^2 = 1 \\quad \\Rightarrow \\quad x^2 - 1 = 1 \\quad \\Rightarrow \\quad x^2 = 2 \\quad \\Rightarrow \\quad x = \\pm \\sqrt{2}\n",
    "     $$\n",
    "\n",
    "### Final Answer:\n",
    "The intersection points of the hyperbola \\( x^2 - y^2 = 1 \\) with the ellipse \\( x^2 + 4y^2 = 6 \\) are:\n",
    "$$\n",
    "(\\sqrt{2}, 1), \\, (-\\sqrt{2}, 1), \\, (\\sqrt{2}, -1), \\, (-\\sqrt{2}, -1)\n",
    "$$\n",
    "\n",
    "https://www.geogebra.org/calculator/y9qyucfb\n",
    "\n",
    "---"
   ]
  },
  {
   "cell_type": "markdown",
   "metadata": {},
   "source": [
    "### Problem: Find the distance between the branches of the hyperbola \\( x^2 - y^2 = 1 \\).\n",
    "\n",
    "1. **Equation of the Hyperbola**:\n",
    "   The given equation of the hyperbola is:\n",
    "   $$\n",
    "   x^2 - y^2 = 1\n",
    "   $$\n",
    "\n",
    "2. **Standard Form of the Hyperbola**:\n",
    "   The standard form of the equation for a hyperbola centered at the origin with horizontal transverse axis is:\n",
    "   $$\n",
    "   \\frac{x^2}{a^2} - \\frac{y^2}{b^2} = 1\n",
    "   $$\n",
    "\n",
    "   Comparing this with the given equation \\( x^2 - y^2 = 1 \\), we can identify \\( a^2 = 1 \\) and \\( b^2 = 1 \\). Therefore, \\( a = 1 \\) and \\( b = 1 \\).\n",
    "\n",
    "3. **Finding the Distance Between the Branches**:\n",
    "   The distance between the two branches of the hyperbola is the distance between the points on the \\( x \\)-axis where the hyperbola intersects. For this, we use the formula for the distance between the branches:\n",
    "   $$\n",
    "   \\text{Distance} = 2a\n",
    "   $$\n",
    "\n",
    "   Since \\( a = 1 \\), the distance between the branches is:\n",
    "   $$\n",
    "   \\text{Distance} = 2 \\times 1 = 2\n",
    "   $$\n",
    "\n",
    "### Final Answer:\n",
    "The distance between the branches of the hyperbola \\( x^2 - y^2 = 1 \\) is \\( 2 \\).\n",
    "\n",
    "https://www.geogebra.org/calculator/ycbqgmup\n",
    "\n",
    "\n",
    "---"
   ]
  },
  {
   "cell_type": "code",
   "execution_count": null,
   "metadata": {
    "vscode": {
     "languageId": "plaintext"
    }
   },
   "outputs": [],
   "source": []
  }
 ],
 "metadata": {
  "language_info": {
   "name": "python"
  }
 },
 "nbformat": 4,
 "nbformat_minor": 2
}
