{
 "cells": [
  {
   "cell_type": "markdown",
   "metadata": {},
   "source": [
    "## Finding the Equation of a Line\n",
    "\n",
    "1. **Formula for the Slope**:  \n",
    "   The slope \\( m \\) of a line passing through two points \\( (x_1, y_1) \\) and \\( (x_2, y_2) \\) is given by:\n",
    "   $$\n",
    "   m = \\frac{y_2 - y_1}{x_2 - x_1}\n",
    "   $$\n",
    "\n",
    "2. **Substitute the Given Points**:  \n",
    "   Here, \\( A(1,2) \\) and \\( B(3,4) \\), so:\n",
    "   $$\n",
    "   m = \\frac{4 - 2}{3 - 1} = \\frac{2}{2} = 1\n",
    "   $$\n",
    "\n",
    "3. **Use the Point-Slope Form**:  \n",
    "   The equation of a line in **point-slope form** is:\n",
    "   $$\n",
    "   y - y_1 = m(x - x_1)\n",
    "   $$\n",
    "   Using point \\( A(1,2) \\):\n",
    "   $$\n",
    "   y - 2 = 1(x - 1)\n",
    "   $$\n",
    "\n",
    "4. **Convert to Slope-Intercept Form**:  \n",
    "   $$\n",
    "   y - 2 = x - 1\n",
    "   $$\n",
    "   $$\n",
    "   y = x + 1\n",
    "   $$\n",
    "\n",
    "**Final Answer**:  \n",
    "The equation of the line is:\n",
    "$$\n",
    "y = x + 1\n",
    "$$\n",
    "\n",
    "https://www.geogebra.org/m/z7cdb5hn\n",
    "\n",
    "---\n"
   ]
  },
  {
   "cell_type": "markdown",
   "metadata": {},
   "source": [
    "## Finding the Equation of a Parallel Line\n",
    "\n",
    "1. **Understanding Parallel Lines**:  \n",
    "   Two lines are **parallel** if they have the **same slope**.  \n",
    "   The given line equation is:\n",
    "   $$\n",
    "   y = 2x + 3\n",
    "   $$\n",
    "   Here, the slope is \\( m = 2 \\).\n",
    "\n",
    "2. **Use the Point-Slope Form**:  \n",
    "   The equation of a line in **point-slope form** is:\n",
    "   $$\n",
    "   y - y_1 = m(x - x_1)\n",
    "   $$\n",
    "   Given that the line passes through \\( A(1,2) \\), we substitute:\n",
    "   $$\n",
    "   y - 2 = 2(x - 1)\n",
    "   $$\n",
    "\n",
    "3. **Convert to Slope-Intercept Form**:  \n",
    "   $$\n",
    "   y - 2 = 2x - 2\n",
    "   $$\n",
    "   $$\n",
    "   y = 2x\n",
    "   $$\n",
    "\n",
    "**Final Answer**:  \n",
    "The equation of the required parallel line is:\n",
    "$$\n",
    "y = 2x\n",
    "$$\n",
    "\n",
    "https://www.geogebra.org/calculator\n",
    "\n",
    "---"
   ]
  },
  {
   "cell_type": "markdown",
   "metadata": {},
   "source": [
    "## Finding the Equation of a Perpendicular Line\n",
    "\n",
    "1. **Understanding Perpendicular Lines**:  \n",
    "   Two lines are **perpendicular** if the product of their slopes is \\( -1 \\).  \n",
    "   The given line equation is:\n",
    "   $$\n",
    "   y = 2x + 3\n",
    "   $$\n",
    "   Here, the slope is \\( m_1 = 2 \\).\n",
    "\n",
    "   The slope \\( m_2 \\) of the line perpendicular to this one satisfies:\n",
    "   $$\n",
    "   m_1 \\times m_2 = -1\n",
    "   $$  \n",
    "   Substituting \\( m_1 = 2 \\), we get:\n",
    "   $$\n",
    "   2 \\times m_2 = -1 \\quad \\Rightarrow \\quad m_2 = -\\frac{1}{2}\n",
    "   $$\n",
    "\n",
    "2. **Use the Point-Slope Form**:  \n",
    "   The equation of a line in **point-slope form** is:\n",
    "   $$\n",
    "   y - y_1 = m(x - x_1)\n",
    "   $$\n",
    "   Given that the line passes through \\( A(1,2) \\) and has slope \\( m_2 = -\\frac{1}{2} \\), we substitute:\n",
    "   $$\n",
    "   y - 2 = -\\frac{1}{2}(x - 1)\n",
    "   $$\n",
    "\n",
    "3. **Convert to Slope-Intercept Form**:  \n",
    "   $$\n",
    "   y - 2 = -\\frac{1}{2}x + \\frac{1}{2}\n",
    "   $$  \n",
    "   $$\n",
    "   y = -\\frac{1}{2}x + \\frac{5}{2}\n",
    "   $$\n",
    "\n",
    "**Final Answer**:  \n",
    "The equation of the required perpendicular line is:\n",
    "$$\n",
    "y = -\\frac{1}{2}x + \\frac{5}{2}\n",
    "$$\n",
    "\n",
    "\n",
    "https://www.geogebra.org/calculator/rfw6kvjx\n",
    "\n",
    "---\n"
   ]
  },
  {
   "cell_type": "markdown",
   "metadata": {},
   "source": [
    "---\n",
    "\n",
    "1. **Given Lines**:\n",
    "\n",
    "We are given the lines:\n",
    "\n",
    "$$\n",
    "y = 2x + 3 \\quad \\text{(Line 1)}\n",
    "$$\n",
    "and\n",
    "$$\n",
    "y = 3x + 2 \\quad \\text{(Line 2)}\n",
    "$$\n",
    "\n",
    "2. **Find the Intersection Point**:\n",
    "\n",
    "To find the intersection point, we set the two equations equal to each other:\n",
    "\n",
    "$$\n",
    "2x + 3 = 3x + 2\n",
    "$$\n",
    "\n",
    "Solve for \\(x\\):\n",
    "\n",
    "$$\n",
    "2x - 3x = 2 - 3\n",
    "$$\n",
    "$$\n",
    "-x = -1\n",
    "$$\n",
    "$$\n",
    "x = 1\n",
    "$$\n",
    "\n",
    "Substitute \\(x = 1\\) into one of the original equations to find \\(y\\):\n",
    "\n",
    "Substitute into \\(y = 2x + 3\\):\n",
    "\n",
    "$$\n",
    "y = 2(1) + 3 = 5\n",
    "$$\n",
    "\n",
    "Thus, the intersection point is:\n",
    "\n",
    "$$\n",
    "\\boxed{(1, 5)}\n",
    "$$\n",
    "\n",
    "3. **Calculate the Angle Between the Lines**:\n",
    "\n",
    "The formula for the angle \\( \\theta \\) between two lines with slopes \\( m_1 \\) and \\( m_2 \\) is:\n",
    "\n",
    "$$\n",
    "\\tan(\\theta) = \\left| \\frac{m_1 - m_2}{1 + m_1 m_2} \\right|\n",
    "$$\n",
    "\n",
    "For Line 1, the slope \\( m_1 = 2 \\), and for Line 2, the slope \\( m_2 = 3 \\).\n",
    "\n",
    "Substitute these values into the formula:\n",
    "\n",
    "$$\n",
    "\\tan(\\theta) = \\left| \\frac{2 - 3}{1 + 2 \\times 3} \\right| = \\left| \\frac{-1}{7} \\right|\n",
    "$$\n",
    "\n",
    "Finally, we can calculate the angle \\( \\theta \\):\n",
    "\n",
    "$$\n",
    "\\theta = \\tan^{-1}\\left( \\frac{1}{7} \\right)\n",
    "$$\n",
    "\n",
    "https://www.geogebra.org/calculator/tc9h7g8k\n",
    "\n",
    "---\n"
   ]
  },
  {
   "cell_type": "markdown",
   "metadata": {},
   "source": [
    "## Finding the Equation of a Parametric Line\n",
    "\n",
    "1. **Understanding Parametric Lines**:  \n",
    "   The parametric form of the equation of a line passing through a point \\( A(x_0, y_0) \\) and parallel to a vector \\( \\mathbf{v} = \\begin{pmatrix} v_1 \\\\ v_2 \\end{pmatrix} \\) is:\n",
    "\n",
    "   $$\n",
    "   \\mathbf{r}(t) = \\mathbf{A} + t \\mathbf{v}\n",
    "   $$\n",
    "\n",
    "   Where:\n",
    "   - \\( \\mathbf{r}(t) = \\begin{pmatrix} x(t) \\\\ y(t) \\end{pmatrix} \\) is the position vector of a point on the line.\n",
    "   - \\( \\mathbf{A} = \\begin{pmatrix} x_0 \\\\ y_0 \\end{pmatrix} \\) is the position vector of the given point.\n",
    "   - \\( t \\) is a parameter.\n",
    "   - \\( \\mathbf{v} = \\begin{pmatrix} v_1 \\\\ v_2 \\end{pmatrix} \\) is the direction vector of the line.\n",
    "\n",
    "### 2. **Substitute the Given Values**:\n",
    "\n",
    "Given \\( A(1, 2) \\) and \\( \\mathbf{v} = \\begin{pmatrix} 2 \\\\ 3 \\end{pmatrix} \\), the equation of the line becomes:\n",
    "\n",
    "$$\n",
    "\\mathbf{r}(t) = \\begin{pmatrix} 1 \\\\ 2 \\end{pmatrix} + t \\begin{pmatrix} 2 \\\\ 3 \\end{pmatrix}\n",
    "$$\n",
    "\n",
    "### 3. **Write the Parametric Equations**:\n",
    "\n",
    "The parametric equations for the line are:\n",
    "\n",
    "$$\n",
    "x(t) = 1 + 2t\n",
    "$$\n",
    "\n",
    "$$\n",
    "y(t) = 2 + 3t\n",
    "$$\n",
    "\n",
    "These equations describe the line passing through point \\( A(1, 2) \\) and parallel to the vector \\( \\mathbf{v} = \\begin{pmatrix} 2 \\\\ 3 \\end{pmatrix} \\).\n",
    "\n",
    "\n",
    "\n",
    "\n",
    "https://www.geogebra.org/calculator/pkzhbdwq\n",
    "\n",
    "---"
   ]
  },
  {
   "cell_type": "markdown",
   "metadata": {},
   "source": [
    "---\n",
    "\n",
    "1. **Parallel Line**:\n",
    "\n",
    "   The equation of the given line is:\n",
    "\n",
    "   $$\n",
    "   y = 2x + 3\n",
    "   $$\n",
    "\n",
    "   A line parallel to this will have the same slope of $2$, but a different y-intercept. For example, using a y-intercept of $-1$, the parallel line is:\n",
    "\n",
    "   $$\n",
    "   y = 2x - 1\n",
    "   $$\n",
    "\n",
    "2. **Perpendicular Line**:\n",
    "\n",
    "   The slope of the given line is $2$, so the slope of the perpendicular line will be the negative reciprocal, which is $-\\frac{1}{2}$.\n",
    "\n",
    "   Let's find the equation of the perpendicular line passing through the point $(1, 0)$. Using the point-slope form:\n",
    "\n",
    "   $$\n",
    "   y - y_1 = m(x - x_1)\n",
    "   $$\n",
    "\n",
    "   Substituting $m = -\\frac{1}{2}$ and $(x_1, y_1) = (1, 0)$:\n",
    "\n",
    "   $$\n",
    "   y - 0 = -\\frac{1}{2}(x - 1)\n",
    "   $$\n",
    "\n",
    "   Simplifying:\n",
    "\n",
    "   $$\n",
    "   y = -\\frac{1}{2}x + \\frac{1}{2}\n",
    "   $$\n",
    "\n",
    "Thus, the parallel line is $y = 2x - 1$, and the perpendicular line is $y = -\\frac{1}{2}x + \\frac{1}{2}$.\n",
    "\n",
    "https://www.geogebra.org/calculator/prjbu2hh\n",
    "\n",
    "---"
   ]
  },
  {
   "cell_type": "markdown",
   "metadata": {},
   "source": [
    "1. **Equation of the Line**:\n",
    "\n",
    "   The given equation of the line is:\n",
    "   $$\n",
    "   y = 2x + 3\n",
    "   $$\n",
    "\n",
    "2. **Convert the Line to Standard Form**:\n",
    "\n",
    "   The general form of the line equation is \\( Ax + By + C = 0 \\). To convert the equation \\( y = 2x + 3 \\) into this form, we rearrange it:\n",
    "   $$\n",
    "   y - 2x - 3 = 0\n",
    "   $$\n",
    "   So, the line is in the form \\( Ax + By + C = 0 \\), where \\( A = -2 \\), \\( B = 1 \\), and \\( C = -3 \\).\n",
    "\n",
    "3. **Formula for the Distance from a Point to a Line**:\n",
    "\n",
    "   The formula for the distance \\( d \\) from a point \\( (x_1, y_1) \\) to a line \\( Ax + By + C = 0 \\) is given by:\n",
    "   $$\n",
    "   d = \\frac{|Ax_1 + By_1 + C|}{\\sqrt{A^2 + B^2}}\n",
    "   $$\n",
    "\n",
    "4. **Substitute the Values**:\n",
    "\n",
    "   For point \\( A(1, 2) \\), we have \\( x_1 = 1 \\) and \\( y_1 = 2 \\). Substituting the values of \\( A = -2 \\), \\( B = 1 \\), and \\( C = -3 \\) into the formula:\n",
    "   $$\n",
    "   d = \\frac{|(-2)(1) + (1)(2) - 3|}{\\sqrt{(-2)^2 + (1)^2}}\n",
    "   $$\n",
    "\n",
    "5. **Simplify**:\n",
    "\n",
    "   First, calculate the numerator:\n",
    "   $$\n",
    "   (-2)(1) + (1)(2) - 3 = -2 + 2 - 3 = -3\n",
    "   $$\n",
    "\n",
    "   Now, calculate the denominator:\n",
    "   $$\n",
    "   \\sqrt{(-2)^2 + (1)^2} = \\sqrt{4 + 1} = \\sqrt{5}\n",
    "   $$\n",
    "\n",
    "   So, the distance is:\n",
    "   $$\n",
    "   d = \\frac{|-3|}{\\sqrt{5}} = \\frac{3}{\\sqrt{5}} = \\frac{3\\sqrt{5}}{5}\n",
    "   $$\n",
    "\n",
    "Thus, the distance from point \\( A(1, 2) \\) to the line \\( y = 2x + 3 \\) is:\n",
    "$$\n",
    "d = \\frac{3\\sqrt{5}}{5}\n",
    "$$\n",
    "\n",
    "https://www.geogebra.org/calculator/zkcaxrjq\n",
    "\n",
    "\n",
    "---"
   ]
  },
  {
   "cell_type": "markdown",
   "metadata": {},
   "source": [
    "### Two-Point Formula for the Equation of a Line\n",
    "\n",
    "Given that the line intersects the coordinate axes at points \\( A(2, 0) \\) and \\( B(0, 3) \\), we can use the **two-point formula** to find the equation of the line.\n",
    "\n",
    "1. **Two-Point Formula**:\n",
    "   The equation of a line passing through points \\( (x_1, y_1) \\) and \\( (x_2, y_2) \\) is:\n",
    "   $$\n",
    "   y - y_1 = \\frac{y_2 - y_1}{x_2 - x_1} (x - x_1)\n",
    "   $$\n",
    "\n",
    "2. **Substitute the Points \\( A(2, 0) \\) and \\( B(0, 3) \\)**:\n",
    "   Substituting \\( x_1 = 2, y_1 = 0, x_2 = 0, y_2 = 3 \\), we get:\n",
    "   $$\n",
    "   y - 0 = \\frac{3 - 0}{0 - 2} (x - 2)\n",
    "   $$\n",
    "\n",
    "3. **Simplify the Equation**:\n",
    "   $$\n",
    "   y = -\\frac{3}{2} (x - 2)\n",
    "   $$\n",
    "\n",
    "4. **Final Equation**:\n",
    "   Expanding and simplifying further:\n",
    "   $$\n",
    "   y = -\\frac{3}{2}x + 3\n",
    "   $$\n",
    "\n",
    "Thus, the equation of the line is:\n",
    "$$\n",
    "y = -\\frac{3}{2}x + 3\n",
    "$$\n",
    "\n",
    "https://www.geogebra.org/calculator/mneqgrnq\n",
    "\n",
    "---"
   ]
  },
  {
   "cell_type": "markdown",
   "metadata": {},
   "source": [
    "### Angle Between a Line and the \\( x \\)-Axis\n",
    "\n",
    "We are given the line equation:\n",
    "\n",
    "$$\n",
    "y = x + 3\n",
    "$$\n",
    "\n",
    "1. **Slope of the Line**:\n",
    "   The slope of the line \\( m \\) is the coefficient of \\( x \\), which is 1. So, we have:\n",
    "\n",
    "$$\n",
    "m = 1\n",
    "$$\n",
    "\n",
    "2. **Formula for the Angle**:\n",
    "   The angle \\( \\theta \\) between the line and the \\( x \\)-axis can be calculated using the formula:\n",
    "\n",
    "$$\n",
    "\\tan(\\theta) = |m|\n",
    "$$\n",
    "\n",
    "Therefore:\n",
    "\n",
    "$$\n",
    "\\theta = \\tan^{-1}(m) = \\tan^{-1}(1)\n",
    "$$\n",
    "\n",
    "3. **Calculate the Angle**:\n",
    "   Using the fact that \\( \\tan^{-1}(1) = 45^\\circ \\), we get:\n",
    "\n",
    "$$\n",
    "\\theta = 45^\\circ\n",
    "$$\n",
    "\n",
    "Thus, the angle between the line \\( y = x + 3 \\) and the \\( x \\)-axis is:\n",
    "\n",
    "$$\n",
    "\\theta = 45^\\circ\n",
    "$$\n",
    "\n",
    "https://www.geogebra.org/calculator/rhmh8jeb\n",
    "\n",
    "---"
   ]
  },
  {
   "cell_type": "markdown",
   "metadata": {},
   "source": [
    "### Perpendicular Vector to the Line \\( x + y + 1 = 0 \\)\n",
    "\n",
    "1. **Line Equation**: \n",
    "   The line equation is:\n",
    "   $$\n",
    "   x + y + 1 = 0\n",
    "   $$\n",
    "\n",
    "2. **Direction Vector of the Line**: \n",
    "   From the line equation \\( x + y + 1 = 0 \\), we can extract the direction vector \\( \\mathbf{v} = \\begin{bmatrix} 1 \\\\ 1 \\end{bmatrix} \\).\n",
    "\n",
    "3. **Perpendicular Vector**: \n",
    "   The vector perpendicular to the line will be the vector that is orthogonal to \\( \\mathbf{v} \\). This can be obtained by swapping the components of the direction vector and changing the sign of one of the components. Thus, the perpendicular vector is:\n",
    "   $$\n",
    "   \\mathbf{v_\\perp} = \\begin{bmatrix} -1 \\\\ 1 \\end{bmatrix}\n",
    "   $$\n",
    "\n",
    "Therefore, a vector perpendicular to the line \\( x + y + 1 = 0 \\) is:\n",
    "$$\n",
    "\\mathbf{v_\\perp} = \\begin{bmatrix} -1 \\\\ 1 \\end{bmatrix}\n",
    "$$\n",
    "\n",
    "\n",
    "https://www.geogebra.org/calculator/ssfwkeuu\n",
    "\n",
    "---"
   ]
  }
 ],
 "metadata": {
  "language_info": {
   "name": "python"
  }
 },
 "nbformat": 4,
 "nbformat_minor": 2
}
